---
title: "Fundamentals of Computational Mathematics - Homework 14"
author: "Jered Ataky"
date: "5/9/2021"
output:
  html_document: default
  pdf_document: default
  word_document: default
---
```{r setup, include=FALSE}
knitr::opts_chunk$set(echo = TRUE)
```

$$
For\ each\ of\ the\ problems,\ we\ are\ going\ to\ use\ this\ Taylor\ expansion\ formula:\\
\\
f( x) \ =\ f( c) +f'( c)( x-c) +\frac{f''( c)}{2!}( x-c)^{2} +\frac{f'''( c)}{3!}( x-c)^{3} +...+\frac{f^{( n)}( c)}{n!}( x-c)^{n}\\
at\ c\ =\ 0\\
\\
f( x) \ =\ f( 0) +f'( 0)( x) +\frac{f''( 0)}{2!}( x)^{2} +\frac{f'''( 0)}{3!}( x)^{3} +...+\frac{f^{( n)}( 0)}{n!}( x)^{n}\\
\\
\\
$$

$$
1.\ f( x) \ =\frac{1}{( 1-x)}\\
\\
f'( x) \ =\ \frac{1}{( 1-x)^{2}} ;\ f''( x) =\frac{2}{( 1-x)^{3}} ;\ f'''( x) =\frac{6}{( 1-x)^{4}} ;\ f^{( iv)} =\frac{24}{( 1-x)^{5}}\\
\\
\\
Therefore:\\
\\
f( x) =1+x+\frac{2}{2!} x^{2} +\frac{6}{3!} x^{3} +\frac{24}{4!} x^{4} +...\\
\\
f( x) \ =\ 1+x+x^{2} +x^{3} +x^{4} +...\\
\\
f( x) =\sum _{n=0}^{\infty } x^{n}\\
\\
\\
$$



$$
2.\ f( x) =e^{x}\\
\\
f( x) =f'( x) =f''( x) =f'''( x) =...=f^{( n)}( x) =e^{x}\\
\\
Therefore:\\
\\
f( x) =1+x+\frac{x^{2}}{2!} +\frac{x^{3}}{3!} +\frac{x^{4}}{4!} +....\\
\\
f( x) =\sum _{n=0}^{\infty }\frac{x^{n}}{n!}\\
\\
\\

$$



$$
3.\ f( x) =ln( 1+x)\\
\\
f'( x) =\frac{1}{1+x} ;\ f''( x) =-\frac{1}{( 1+x)^{2}} ;\ f'''( x) =\frac{2}{( 1+x)^{3}} ;\ f^{( iv)}( x) =-\frac{6}{( 1+x)^{4}}\\
\\
f( x) =0+x-\frac{x^{2}}{2!} +\frac{2}{3!} x^{3} -\frac{6}{4!} x^{4} +...\\
\\
f( x) =\frac{x}{1} -\frac{x^{2}}{2} +\frac{x^{3}}{3} -\frac{x^{4}}{4} +...\\
\\
\\
f( x) =\sum _{n=1}^{\infty }( -1)^{n+1}\frac{x^{n}}{n}\\
\\
$$



